lambda2Gmu/Tests2.v
@@ -1,0 +1,77 @@
+Require Import Definitions.
+Require Import TLC.LibLN.
+
+(* TODO merge with Tests.v *)
+
+Notation "@ n" := (typ_bvar n) (at level 42).
+Notation "# n" := (trm_bvar n) (at level 42).
+Ltac fs := exact \{}. (* There must be a better way *)
+
+Axiom Nat : var.
+Definition NatDef := GADT 0 [
+                            GADTconstr 0 typ_unit (typ_gadt [] Nat);
+                            GADTconstr 0 (typ_gadt [] Nat) (typ_gadt [] Nat)
+                          ].
+
+Ltac ininv :=
+  match goal with
+  | H: List.In _ _ |- _ =>
+    inversions H
+  end.
+
+Definition natSigma := (empty & Nat ~ NatDef).
+
+Lemma oknat : okGadt natSigma.
+  constructor*.
+  - constructor.
+  - intros; repeat ininv.
+    + econstructor.
+      * intros. destruct Alphas; inversions H; econstructor.
+      * intros. destruct Alphas; inversions H; econstructor.
+        intros.
+        inversion H.
+        auto. auto.
+      * auto.
+    + econstructor.
+      * intros. destruct Alphas; inversions H; econstructor.
+        intros.
+        inversion H.
+        auto. auto.
+      * intros. destruct Alphas; inversions H; econstructor.
+        intros.
+        inversion H.
+        auto. auto.
+      * auto.
+        Unshelve. fs. fs.
+Qed.
+
+Definition zero := trm_constructor [] (Nat, 0) trm_unit.
+
+Lemma zero_type : {natSigma, empty} ⊢ zero ∈ typ_gadt [] Nat.
+  cbv.
+  econstructor; eauto.
+  - cbn.
+    instantiate (3:=0).
+    cbn.
+    eauto.
+  - econstructor.
+    econstructor. apply oknat.
+  - cbv. eauto.
+Qed.
+
+Definition succ := trm_abs (typ_gadt [] Nat) (trm_constructor [] (Nat, 1) (#0)).
+
+Lemma succ_type : {natSigma, empty} ⊢ succ ∈ (typ_gadt [] Nat) ==> (typ_gadt [] Nat).
+  cbv.
+  econstructor.
+  intros.
+  econstructor; eauto.
+  - cbn. instantiate (3:=0); cbn. eauto.
+  - cbv. case_if.
+    econstructor; eauto.
+    econstructor; eauto.
+    econstructor. apply oknat.
+    econstructor; eauto.
+    intros. inversions H0.
+  - cbn. auto.
+Qed.
